new opt

hol/policy_to_table/fwd_proofLib.sig
@@ -3,5 +3,5 @@ sig
   include Abbrev
 
         val convert_arith_policy_to_interval_tables : term * term * term * term * term -> thm
-
+        val time_stage : string * Timer.cpu_timer * Timer.real_timer -> {sys: Time.time, usr: Time.time} * Time.time
 end
