hol/policy_to_table/tables_spec_newScript.sml
@@ -1,0 +1,266 @@
+open HolKernel boolLib liteLib simpLib Parse bossLib;
+open arithmeticTheory stringTheory containerTheory pred_setTheory
+     listTheory finite_mapTheory;
+
+open p4Lib;
+open blastLib bitstringLib;
+open p4Theory;
+open p4_auxTheory;
+open p4_coreTheory;
+
+open bitstringTheory;
+open wordsTheory;
+open optionTheory;
+open sumTheory;
+open stringTheory;
+open ottTheory;
+open pairTheory;
+open rich_listTheory;
+open arithmeticTheory;
+open alistTheory;
+open numeralTheory;
+open alistTheory;
+open set_relationTheory;
+open pred_setTheory;
+open pred_setLib;
+
+open bdd_genTheory;     
+open pred_specTheory;     
+open policy_specTheory;     
+     
+open tables_specTheory;
+
+val _ = new_theory "tables_spec_new";
+
+    
+
+
+(* table simplifications *)
+
+
+(*
+examples of checks:
+1. how many times we call?
+When is it final?
+
+mk_bdd 
+
+*)
+
+
+
+(*)
+Definition simp_row_new_def:
+  simp_row_new atoml =
+  let simplified_row = MAP (\atom. simp_atom atom) atoml in
+    let simplified_row' = FILTER (\x. is_not_true_var_atom x) simplified_row in
+    case MEM False simplified_row' of
+    | T => [False]
+    | F => (
+
+      FILTER (\x. is_not_true_var_atom x) simplified_row
+    )
+End
+*)
+
+(*
+Definition simp_row_new_def:
+  (simp_row_new [] = [True]) /\
+  (simp_row_new (a::atoml) =
+  let sa = simp_atom a in
+  (case sa of
+   | False => [False]
+   | True => simp_row_new atoml
+   | _ => sa ::( simp_row_new atoml)
+  )
+  )
+End
+
+
+
+Definition simp_tbl_new_def:
+  simp_tbl_new ([]: 'a var_table) = [] /\
+  simp_tbl_new ((atom,st,res)::tbl) = 
+  let atom' = simp_row_new atom in
+  case atom' of
+  | [False] => simp_tbl_new tbl
+  | [True] => [([True],st,res)]
+  | _ => (atom',st,res)::(simp_tbl_new tbl) 
+End
+
+
+
+(*
+Definition simp_tbl_new_def:
+  simp_tbl_new (tbl: 'a var_table) =
+  let st = MAP (\(atoml,st_num,res). simp_row_new atoml,st_num,res) tbl in
+    FILTER (\(atoml,st,res). atoml <> [False]) st
+End
+*)
+
+Definition simp_tbll_new_def:
+  simp_tbll_new (tbll: 'a var_table_list) =
+   MAP (\tbl. simp_tbl_new tbl) tbll
+End
+
+
+Definition simp_tables_new_def:
+  simp_tables_new ((tbll: 'a var_table_list), st_in) =
+   (simp_tbll_new tbll, st_in:num)
+End
+ 
+*)
+
+
+
+Definition is_not_true_var_atom_def:
+  (is_not_true_var_atom True = F) /\
+  (is_not_true_var_atom _ = T)
+End
+
+
+
+Definition simp_row_new_def:
+  simp_row_new atoml =
+  let simp_row = MAP (\atom. simp_atom atom) atoml in
+    let simp_row' = FILTER (\x. is_not_true_var_atom x) simp_row in
+      case simp_row' of
+      | [] => [True]
+      | _ => 
+          (case MEM False simp_row' of
+           | T => [False]
+           | F => simp_row')
+End
+
+
+        
+
+
+
+Definition simp_table_new_def:
+  (simp_table_new [] s = []) ∧
+                  
+  (simp_table_new ((atoms,st,res)::table)  NONE =
+   let atoms' = simp_row_new atoms in
+     case atoms' of
+     | [False] => simp_table_new table NONE
+     | _ =>  ((atoms', st, res)::simp_table_new table NONE)
+  ) ∧
+    
+  (simp_table_new ((atoms,st,res)::table) (SOME s') =
+   if (s' ≠ st) then
+     simp_table_new table (SOME s')
+   else
+     (
+     let atoms' = simp_row_new atoms in
+       case atoms' of
+       | [False] => simp_table_new table (SOME s')
+       | [True] => [(atoms', st, res)]
+       | _ =>  ((atoms', st, res) :: (simp_table_new table (SOME s')))
+     )
+  )
+End
+
+
+
+                        
+
+
+Definition simp_tables_new_def:
+  (simp_tables_new [] s = []) ∧
+  (simp_tables_new (t::table) s = 
+   (let t' = simp_table_new t s in
+      ( case t' of
+        | [([True], s , state s'')] => (t'::(simp_tables_new table (SOME s'')))
+        | _ => (t'::(simp_tables_new table NONE))
+      )
+   )
+  )
+End
+
+
+
+
+Definition simp_tables_wrapper_new_def:
+  simp_tables_wrapper_new ((tbll: 'a var_table_list), st_in) =
+   (simp_tables_new tbll (SOME st_in), st_in)
+End
+
+
+
+
+
+
+(*****************************)
+
+
+Definition final_row_new_def:
+  (final_row_new ([],_,_) s = NONE) ∧
+  (final_row_new ([True], s', s'') s = (if s = s' then SOME s'' else NONE)) ∧
+  (final_row_new _ s = NONE)
+End
+        
+
+
+
+Definition final_tbl_new_def:
+  (final_tbl_new [] s = NONE) ∧
+  (final_tbl_new (row::rows) s =         
+     case final_row_new row s of
+       SOME a => SOME a
+     | NONE => if (FST row = [False]) then final_tbl_new rows s else NONE
+  )
+End
+
+
+
+Definition final_tbll_new_def:
+  final_tbll_new ([]: 'a var_table_list) st_in = NONE ∧
+  final_tbll_new [tbl] st_in =
+  ( case final_tbl_new tbl st_in of
+    | SOME (action a) => SOME (action a)
+    | _ => NONE       
+  )∧
+  final_tbll_new (tbl::tbls) st_in =
+  ( case final_tbl_new tbl st_in of
+    | SOME (state n) => final_tbll tbls n
+    | _ => NONE
+  )
+End
+
+
+Definition final_tables_new_def:
+  final_tables_new (tbll, st_in) =
+  final_tbll_new tbll st_in
+End
+
+
+
+
+
+
+
+
+
+        
+
+
+Definition table_structure_new_def:
+  table_structure_new =
+  <|
+    sem := sem_tables;
+    sub := mk_substitute_tables;
+    simp := simp_tables_wrapper_new;
+    final := final_tables_new;
+    fv := fv_tables;
+  |>
+End            
+
+
+
+
+
+                 
+val _ = export_theory ();
+
+    
